IterAssocOp : proved iter_op with function exponential

src/Util/IterAssocOp.v
@@ -7,7 +7,9 @@ Section IterAssocOp.
   Context `{Equivalence T}
           (op:T->T->T) {op_proper:Proper (equiv==>equiv==>equiv) op}
           (assoc: forall a b c, op a (op b c) === op (op a b) c)
-          (neutral:T) (neutral_neutral : forall a, op a neutral === a).
+          (neutral:T)
+          (neutral_l : forall a, op neutral a === a)
+          (neutral_r : forall a, op a neutral === a).
   Existing Instance op_proper.
 
   Fixpoint nat_iter_op n a :=
@@ -15,6 +17,12 @@ Section IterAssocOp.
     | 0%nat => neutral
     | S n' => op a (nat_iter_op n' a)
     end.
+
+  Lemma nat_iter_op_plus : forall m n a,
+    op (nat_iter_op m a) (nat_iter_op n a) === nat_iter_op (m + n) a.
+  Proof.
+    induction m; intros; simpl; rewrite ?neutral_l, <-?IHm, ?assoc; reflexivity.
+  Qed.
 
   Definition N_iter_op n a :=
     match n with
@@ -29,11 +37,149 @@ Section IterAssocOp.
 
   Lemma N_iter_op_succ : forall n a, N_iter_op (N.succ n) a  === op a (N_iter_op n a).
   Proof.
-    destruct n; simpl; intros; rewrite ?Pos_iter_op_succ, ?neutral_neutral; reflexivity.
+    destruct n; simpl; intros; rewrite ?Pos_iter_op_succ, ?neutral_r; reflexivity.
   Qed.
 
   Lemma N_iter_op_is_nat_iter_op : forall n a, N_iter_op n a === nat_iter_op (N.to_nat n) a.
   Proof.
     induction n using N.peano_ind; intros; rewrite ?N2Nat.inj_succ, ?N_iter_op_succ, ?IHn; reflexivity.
   Qed.
+
+  Fixpoint funexp {A} (f : A -> A) (a : A) (exp : nat) : A :=
+    match exp with
+    | O => a
+    | S exp' => f (funexp f a exp')
+    end.
+
+  Definition test_and_op n a (state : nat * T) :=
+    let '(i, acc) := state in
+    let acc2 := op acc acc in
+    match i with
+    | O => (0, acc)
+    | S i' => (i', if N.testbit_nat n i' then op a acc2 else acc2)
+    end.
+
+  Definition iter_op n a : T := 
+    snd (funexp (test_and_op n a) (N.size_nat n, neutral) (N.size_nat n)).
+
+  Definition test_and_op_inv n a (s : nat * T) :=
+    snd s === nat_iter_op (N.to_nat (N.shiftr_nat n (fst s))) a.
+
+  Hint Rewrite
+    N.succ_double_spec
+    N.add_1_r
+    Nat2N.inj_succ
+    Nat2N.inj_mul
+    N2Nat.id: N_nat_conv
+ .
+
+  Lemma Nsucc_double_to_nat : forall n,
+    N.succ_double n = N.of_nat (S (2 * N.to_nat n)).
+  Proof.
+    intros.
+    replace 2 with (N.to_nat 2) by auto.
+    autorewrite with N_nat_conv.
+    reflexivity.
+  Qed.
+
+  Lemma Ndouble_to_nat : forall n,
+    N.double n = N.of_nat (2 * N.to_nat n).
+  Proof.
+    intros.
+    replace 2 with (N.to_nat 2) by auto.
+    autorewrite with N_nat_conv.
+    reflexivity.
+  Qed.
+
+  Lemma shiftr_succ : forall n i,
+    N.to_nat (N.shiftr_nat n i) =
+    if N.testbit_nat n i
+    then S (2 * N.to_nat (N.shiftr_nat n (S i)))
+    else (2 * N.to_nat (N.shiftr_nat n (S i))).
+  Proof.
+    intros.
+    rewrite Nshiftr_nat_S.
+    case_eq (N.testbit_nat n i); intro testbit_i;
+      pose proof (Nshiftr_nat_spec n i 0) as shiftr_n_odd;
+      rewrite Nbit0_correct in shiftr_n_odd; simpl in shiftr_n_odd;
+      rewrite testbit_i in shiftr_n_odd.
+    + pose proof (Ndiv2_double_plus_one (N.shiftr_nat n i) shiftr_n_odd) as Nsucc_double_shift.
+      rewrite Nsucc_double_to_nat in Nsucc_double_shift.
+      apply Nat2N.inj.
+      rewrite Nsucc_double_shift.
+      apply N2Nat.id.
+    + pose proof (Ndiv2_double (N.shiftr_nat n i) shiftr_n_odd) as Nsucc_double_shift.
+      rewrite Ndouble_to_nat in Nsucc_double_shift.
+      apply Nat2N.inj.
+      rewrite Nsucc_double_shift.
+      apply N2Nat.id.
+  Qed.
+
+  Lemma test_and_op_inv_step : forall n a s,
+    test_and_op_inv n a s ->
+    test_and_op_inv n a (test_and_op n a s).
+  Proof.
+    destruct s as [i acc].
+    unfold test_and_op_inv, test_and_op; simpl; intro Hpre.
+    destruct i; [ apply Hpre | ].
+    simpl.
+    rewrite shiftr_succ.
+    case_eq (N.testbit_nat n i); intro; simpl; rewrite Hpre, <- plus_n_O, nat_iter_op_plus; reflexivity.
+  Qed.
+
+  Lemma test_and_op_inv_holds : forall n a i s,
+    test_and_op_inv n a s ->
+    test_and_op_inv n a (funexp (test_and_op n a) s i).
+  Proof.
+    induction i; intros; auto; simpl; apply test_and_op_inv_step; auto.
+  Qed.
+
+  Lemma funexp_test_and_op_index : forall n a x acc y,
+    fst (funexp (test_and_op n a) (x, acc) y) === x - y.
+  Proof.
+    induction y; simpl; rewrite <- ?Minus.minus_n_O; try reflexivity.
+    destruct (funexp (test_and_op n a) (x, acc) y) as [i acc'].
+    simpl in IHy.
+    unfold test_and_op.
+    destruct i; rewrite NPeano.Nat.sub_succ_r; subst; rewrite <- IHy; simpl; reflexivity.
+  Qed.
+
+  Lemma iter_op_termination : forall n a,
+    test_and_op_inv n a 
+      (funexp (test_and_op n a) (N.size_nat n, neutral) (N.size_nat n)) -> 
+    iter_op n a === nat_iter_op (N.to_nat n) a.
+  Proof.
+    unfold test_and_op_inv, iter_op; simpl; intros ? ? Hinv.
+    rewrite Hinv, funexp_test_and_op_index, Minus.minus_diag.
+    replace (N.shiftr_nat n 0) with n by auto.
+    reflexivity.
+  Qed.
+
+  Lemma Nsize_nat_equiv : forall n, N.size_nat n = N.to_nat (N.size n).
+  Proof.
+    destruct n; auto; simpl; induction p; simpl; auto; rewrite IHp, Pnat.Pos2Nat.inj_succ; reflexivity.
+  Qed.
+
+  Lemma Nshiftr_size : forall n, N.shiftr_nat n (N.size_nat n) = 0%N.
+  Proof.
+    intros.
+    rewrite Nsize_nat_equiv.
+    rewrite Nshiftr_nat_equiv.
+    destruct (N.eq_dec n 0); subst; auto.
+    apply N.shiftr_eq_0.
+    rewrite N.size_log2 by auto.
+    apply N.lt_succ_diag_r.
+  Qed.
+  
+  Lemma iter_op_spec : forall n a, iter_op n a === nat_iter_op (N.to_nat n) a.
+  Proof.
+    intros.
+    apply iter_op_termination.
+    apply test_and_op_inv_holds.
+    unfold test_and_op_inv.
+    simpl.
+    rewrite Nshiftr_size.
+    reflexivity.
+  Qed.
+
 End IterAssocOp.
